Try to let normalize work with parameterized instance. Fail with a Module namespace issue. Commit to try new approach.

LogicGenerator/demo/implementation_6.v
@@ -1,17 +1,30 @@
 Require Import HypotheticalExternLib.
 Require Import ZArith.
-Require Import interface_1.
+Require Import interface_6.
 
 Module NaiveLang.
-  Definition expr {p: para} := (nat -> X * X) -> Prop.
+  Definition expr `{para} := (nat -> option X) -> Prop.
   Section NaiveLang.
-  Context {p: para}.
+  Context `{para}.
   Definition context := expr -> Prop.
   Definition impp (e1 e2 : expr) : expr := fun st => e1 st -> e2 st.
   Definition andp (e1 e2 : expr) : expr := fun st => e1 st /\ e2 st.
   Definition orp  (e1 e2 : expr) : expr := fun st => e1 st \/ e2 st.
   Definition falsep : expr := fun st => False.
+  Definition coq_prop (P: Prop): expr := fun _ => P.
 
+  Definition join : (nat -> option X) -> (nat -> option X) -> (nat -> option X) -> Prop :=
+    fun x y z =>
+      forall p: nat,
+       (exists v, x p = Some v /\ y p = None /\ z p = Some v) \/
+       (exists v, x p = None /\ y p = Some v /\ z p = Some v) \/
+       (x p = None /\ y p = None /\ z p = None).
+  Definition sepcon (e1 e2 : expr) : expr := fun st =>
+    exists st1 st2, join st1 st2 st /\ e1 st1 /\ e2 st2.
+  Definition emp : expr := fun st =>
+    forall p, st p = None.
+  Definition corable (e: expr): Prop := forall s1 s2, e s1 <-> e s2.
+  
   Definition provable (e : expr) : Prop := forall st, e st.
   End NaiveLang.
 End NaiveLang.
@@ -19,7 +32,8 @@ End NaiveLang.
 Module NaiveRule.
   Include DerivedNames (NaiveLang).
   Section NaiveRule.
-  Context {p: para}.
+  Context `{para}.
+
   Lemma modus_ponens :
     forall x y : expr, provable (impp x y) -> provable x -> provable y.
   Proof. unfold provable, impp. auto. Qed.
@@ -56,6 +70,26 @@ Module NaiveRule.
 
   Lemma excluded_middle : forall x : expr, provable (orp x (negp x)).
   Proof. unfold provable, orp, negp, impp, falsep. intros; tauto. Qed.
+
+  Lemma coq_prop_intros : (forall P : Prop, P -> provable (coq_prop P)) .
+  Proof. unfold provable, coq_prop. intros; tauto. Qed.
+  
+  Lemma coq_prop_elim : (forall (P : Prop) (x : expr), (P -> provable x) -> provable (impp (coq_prop P) x)) .
+  Proof. unfold provable, impp, coq_prop. intros; auto. Qed.
+    
+  Lemma coq_prop_impp : (forall P Q : Prop, provable (impp (impp (coq_prop P) (coq_prop Q)) (coq_prop (P -> Q)))) .
+  Proof. unfold provable, impp, coq_prop. intros; auto. Qed.
+  
+  Axiom sepcon_comm: forall x y, provable (iffp (sepcon x y) (sepcon y x)).
+  Axiom sepcon_assoc: forall x y z,
+      provable (iffp (sepcon x (sepcon y z)) (sepcon (sepcon x y) z)).
+  Axiom sepcon_mono : (forall x1 x2 y1 y2 : expr, provable (impp x1 x2) -> provable (impp y1 y2) -> provable (impp (sepcon x1 y1) (sepcon x2 y2))) .
+  Axiom sepcon_emp : (forall x : expr, provable (iffp (sepcon x emp) x)) .
+  Axiom falsep_sepcon_left : (forall x : expr, provable (impp (sepcon falsep x) falsep)) .
+  Axiom orp_sepcon_left : (forall x y z : expr, provable (impp (sepcon (orp x y) z) (orp (sepcon x z) (sepcon y z)))) .
+  Axiom corable_coq_prop : (forall P : Prop, corable (coq_prop P)) .
+  Axiom corable_preserved' : (forall x y : expr, provable (iffp x y) -> corable x -> corable y) .
+  Axiom corable_andp_sepcon1 : (forall x y z : expr, corable x -> provable (iffp (sepcon (andp x y) z) (andp x (sepcon y z)))) .
   End NaiveRule.
 End NaiveRule.
 
@@ -64,11 +98,4 @@ Module Solver := IPSolver NaiveLang.
 Import T.
 Import Solver.
 
-Notation "x --> y" := (impp x y)(at level 55, right associativity).
-Notation "x && y" := (andp x y)(at level 40, left associativity).
-Notation "|-- P " := (provable P) (at level 71, no associativity).
 
-Goal forall {p: para} (P Q R: (nat -> X * X) -> Prop), |-- Q && P --> R --> P && Q && R.
-  intros.
-  Fail ip_solve.
-Abort.
