LogicGenerator/demo/configuration_6.v
@@ -3,7 +3,7 @@ Local Open Scope string.
 
 Definition instance_para_open := true.
 Definition local_lib_file := "HypotheticalExternLib".
-Definition implementation_file := "implementation_1".
+Definition implementation_file := "implementation_6".
 Definition result_module := "T".
 Definition instance_para := "para".
 
@@ -18,15 +18,21 @@ Definition how_connectives :=
   ;primitive_connective andp
   ;primitive_connective orp
   ;primitive_connective falsep
+  ;primitive_connective coq_prop
+  ;primitive_connective sepcon
+  ;primitive_connective emp
   ;FROM_andp_impp_TO_iffp
   ;FROM_falsep_impp_TO_negp
   ;FROM_falsep_impp_TO_truep
   ;FROM_impp_TO_multi_imp
   ;FROM_empty_set_TO_empty_context
+  ;FROM_andp_TO_iter_andp
+  ;FROM_sepcon_TO_iter_sepcon
   ].
 
 Definition how_judgements :=
   [primitive_judgement provable
+  ;primitive_judgement corable
   ;FROM_provable_TO_derivable
   ].
 
@@ -37,5 +43,12 @@ Definition primitive_rule_classes :=
   [ provability_OF_impp
   ; provability_OF_propositional_connectives
   ; provability_OF_classical_logic
+  ; provability_OF_coq_prop
+  ; provability_OF_sepcon_rule_AS_weak_iffp
+  ; provability_OF_sepcon_rule_AS_mono
+  ; provability_OF_sepcon_orp_rule
+  ; provability_OF_sepcon_falsep_rule
+  ; provability_OF_emp_rule_AS_iffp
+  ; corability_OF_basic_setting
+  ; corability_OF_coq_prop
   ].
-
