LogicGenerator/demo/test_6.v
@@ -1,0 +1,39 @@
+Require Import Logic.ExportSolvers.Normalize_Para.
+Require Import HypotheticalExternLib.
+Require Import interface_6.
+Require Import implementation_6.
+Require Import export_lib_6.
+
+Module T.
+Include DerivedNames (NaiveLang).
+Include BETA.
+End T.
+
+Module Tac := ExportTactic T.
+
+Parameter p: para.
+Existing Instance p.
+
+Local Declare Scope syntax.
+Local Open Scope syntax.
+
+Import T.
+Import Tac.
+
+Notation "|--  x" := (provable x) (at level 71, no associativity) : syntax.
+Notation "'!!' e" := (coq_prop e) (at level 25) : syntax.
+Notation "x && y" := (andp x y) (at level 40, left associativity) : syntax.
+Notation "x <--> y" := (iffp x y) (at level 60, no associativity) : syntax.
+Notation "x --> y" := (impp x y) (at level 55, right associativity) : syntax.
+Notation "x * y" := (sepcon x y) (at level 40, left associativity) : syntax.
+
+Goal forall (P: Prop) (Q R S: (nat -> option X) -> Prop),
+  |-- (!! P && Q) * R * S --> (!! P && Q) * (!! P && R) * (!! P && S).
+Proof.
+  intros.
+  normalize.
+  Search Morphisms.Proper sepcon.
+  match goal with
+  | |- context [ !! ?P && ?Q * ?R ] => pose proof (prop_andp_sepcon1 P Q R)
+  end.
+Print Ltac normalize1.
